code/experimental/P256/Hacl.Impl.P256.LowLevel.fst
@@ -60,6 +60,30 @@ let lemma_t_computation2 t =
   assert_norm(18446744073709551615 + 4294967295 * pow2 64 + 18446744069414584321 * pow2 192 = prime256)
 
 
+val p256_add: arg1: felem -> arg2: felem ->  out: felem -> Stack unit 
+  (requires (fun h0 ->  
+    live h0 arg1 /\ live h0 arg2 /\ live h0 out /\ 
+    eq_or_disjoint arg1 out /\ eq_or_disjoint arg2 out /\
+    as_nat h0 arg1 < prime256 /\ as_nat h0 arg2 < prime256 
+   )
+  )
+  (ensures (fun h0 _ h1 -> modifies1 out h0 h1 /\ 
+      as_nat h1 out == (as_nat h0 arg1 + as_nat h0 arg2) % prime256 /\
+      as_seq h1 out == felem_add_seq (as_seq h0 arg1) (as_seq h0 arg2)
+  ))
+
+
+let p256_add arg1 arg2 out = 
+  let h0 = ST.get() in   
+  let t = add4 arg1 arg2 out in 
+    lemma_t_computation t;
+    reduction_prime256_2prime256_with_carry_impl t out out;
+  let h2 = ST.get() in 
+    additionInDomain2Nat (as_nat h0 arg1) (as_nat h0 arg2);
+    inDomain_mod_is_not_mod (fromDomain_ (as_nat h0 arg1) + fromDomain_ (as_nat h0 arg2));
+    lemma_eq_funct (as_seq h2 out) (felem_add_seq (as_seq h0 arg1) (as_seq h0 arg2))
+
+
 val p256_double: arg1: felem ->  out: felem -> Stack unit 
   (requires (fun h0 ->  live h0 arg1 /\ live h0 out /\ eq_or_disjoint arg1 out /\ as_nat h0 arg1 < prime256))
   (ensures (fun h0 _ h1 -> modifies1 out h0 h1 /\ as_nat h1 out == (2 * as_nat h0 arg1) % prime256 /\ as_nat h1 out < prime256))
@@ -76,14 +100,8 @@ val p256_sub: arg1: felem -> arg2: felem -> out: felem -> Stack unit
       eq_or_disjoint arg1 out /\ eq_or_disjoint arg2 out /\
       as_nat h0 arg1 < prime256 /\ as_nat h0 arg2 < prime256))
     (ensures (fun h0 _ h1 -> modifies1 out h0 h1 /\ 
-      (
-	(*let x = as_seq h0 arg1 in 
-	let y = as_seq h0 arg2 in 
-	let out = as_seq h1 out in 
-	felem_seq_as_nat out == (felem_seq_as_nat x - felem_seq_as_nat y) % prime256 /\ *)
 	as_nat h1 out == (as_nat h0 arg1 - as_nat h0 arg2) % prime256 /\
 	as_seq h1 out == felem_sub_seq (as_seq h0 arg1) (as_seq h0 arg2)
-      )
   ))
 
 let p256_sub arg1 arg2 out = 
